Steel.Kont: using a layered effect

ulib/experimental/Steel.Kont.fst
@@ -11,8 +11,23 @@ open Steel.Primitive.ForkJoin
 
 module U = FStar.Universe
 
+assume val l_assoc : unit -> Lemma (forall h1 h2 h3. star (star h1 h2) h3 `equiv` star h1 (star h2 h3))
+assume val l_comm : unit -> Lemma (forall h1 h2. star h1 h2 `equiv` star h2 h1)
+assume val l_id : unit -> Lemma (forall h. star h emp `equiv` h /\ star emp h `equiv` h)
+assume val l_frame : unit -> Lemma (forall h1 h2 h3. equiv h1 h2 ==> equiv (star h1 h3) (star h2 h3))
 
-//assume val sorry : #a:Type -> #p:_ -> #q:_ -> unit -> SteelT a p q
+(* Some helpers *)
+private
+val reshuffle0 (#p #q : hprop)
+              (_ : squash (p `equiv` q))
+   : SteelT unit p (fun _ -> q)
+
+private
+let reshuffle0 #p #q peq =
+  Steel.SteelAtomic.Basics.lift_atomic_to_steelT
+    (fun () -> Steel.Effect.Atomic.change_hprop p q (fun m -> ()))
+
+assume val sorry : #a:Type -> #p:_ -> #q:_ -> unit -> SteelT a p q
 
 let ret #a (x:a) : SteelT a emp (fun _ -> emp) =
   Steel?.reflect (returnc _ x (fun _ -> emp)) // expected that I need to do this instead of just `x`?
@@ -28,44 +43,118 @@ type steelK (t:Type) (pre : hprop) (post:post_t t) =
   SteelT unit (frame `star` pre) (fun _ -> postf)
 
 (* The classic continuation monad *)
-let return #a (x:a) : steelK a emp (fun _ -> emp) =
+let return a (x:a) : steelK a emp (fun _ -> emp) =
   fun k -> k x
 
-let bind #a #b #pre #post #post'
+let bind a b pre post post'
   (m : steelK a pre post)
   (f : (x:a -> steelK b (post x) post'))
   : steelK b pre post'
  = fun k -> m (fun x -> f x k)
+ 
+let himplies h1 h2 =
+  forall m. interp h1 m ==> interp h2 m
 
-(* Identity cont with frame, to eliminate a steelK *)
+(* Helper. Needed because of #1948 mostly *)
+let change_pre #a #b #pre1 #pre2 #post
+  (f : (x:b -> SteelT a (pre1 x) (post x)))
+  : Pure (x:b -> SteelT a (pre2 x) (post x)) (requires (forall x. pre1 x `equiv` pre2 x)) (ensures (fun _ -> True))
+  = fun x -> reshuffle0 (); f x
+
+(* How does this not exist in FStar.Classical?? *)
+let forall_elim #a (#p:a -> Type0) ($l : unit -> Lemma (forall x. p x)) (x:a) : Lemma (p x) = l ()
+let forall_elim_2 #a #b (#p:a -> b -> Type0) ($l : unit -> Lemma (forall x y. p x y)) (x:a) (y:b) : Lemma (p x y) = l ()
+let forall_elim_3 #a #b #c (#p:a -> b -> c -> Type0) ($l : unit -> Lemma (forall x y z. p x y z)) (x:a) (y:b) (z:c) : Lemma (p x y z) = l ()
+
+(* Only deals with equivalences really *)
+let subcomp (a:Type) pre1 pre2 post1 post2 (f : steelK a pre1 post1)
+    : Pure (steelK a pre2 post2)
+           (requires (pre2 `equiv` pre1 /\ (forall x. post1 x `equiv` post2 x)))
+           (ensures (fun _ -> True)) =
+  fun #frame #postf (k : (x:a -> SteelT unit (frame `star` (post2 x)) (fun _ -> postf))) ->
+  forall_elim_3 l_frame pre1 pre2 frame;
+  forall_elim_2 l_comm pre1 frame;
+  forall_elim_2 l_comm pre2 frame;
+  let aux (x:a) : Lemma ((frame `star` post1 x) `equiv` (frame `star` post2 x)) =
+    forall_elim_3 l_frame (post1 x) (post2 x) frame;
+    forall_elim_2 l_comm (post1 x) frame;
+    forall_elim_2 l_comm (post2 x) frame
+  in
+  FStar.Classical.forall_intro aux;
+  change_pre (f #frame #postf) (change_pre k)
+
+let refine_mprop_const #fp (phi:prop) : refine_mprop fp =
+  fun _ -> phi
+
+let if_then_else (a:Type u#aa) pre1 pre2 post1 post2
+                 (f : steelK a pre1 post1)
+                 (g : steelK a pre2 post2)
+                 (p:Type0) : Type =
+  let p : prop = squash p in
+  let rp = refine_mprop_const p in
+  let rnp = refine_mprop_const (~p) in
+  steelK a ((refine pre1 rp) `h_or` (refine pre2 rnp))
+           (fun x -> ((refine (post1 x) rp) `h_or` (refine (post2 x) rnp)))
+
+#push-options "--admit_smt_queries true" // todo: revise
+reifiable reflectable
+layered_effect {
+  SteelK : a:Type -> pre:pre_t -> post:(post_t a) -> Effect
+  with
+  repr = steelK;
+  return = return;
+  bind = bind;
+  subcomp = subcomp;
+  if_then_else = if_then_else
+}
+#pop-options
+
+assume val ksorry : #a:Type -> #p:_ -> #q:_ -> unit -> SteelK a p q
+
+assume Pure_wp_monotonic:
+  (forall (a:Type) (wp:pure_wp a).
+     (forall p q. (forall x. p x ==> q x) ==>
+             (wp p ==> wp q)))
+
+let lift_pure_SteelK (a:Type) (wp:pure_wp a)
+                     (p:hprop)
+                     (f : unit -> PURE a wp)
+                     : Pure (steelK a p (fun _ -> p)) (requires (wp (fun _ -> True))) (ensures (fun _ -> True))
+  = (fun k -> k (f ()))
+
+sub_effect PURE ~> SteelK = lift_pure_SteelK
+
+(* Sanity check *)
+let test_lift #p #q (f : unit -> SteelK unit p (fun _ -> q)) : SteelK unit p (fun _ -> q) =
+  ();
+  f ();
+  ()
+
+(* Identity cont with frame, to eliminate a SteelK *)
 let idk #frame #a (x:a) : SteelT a frame (fun x -> frame) =
   Steel?.reflect (returnc _ x (fun _ -> frame))
 
-(* Helper. Needed because of #1948 mostly *)
-let change_pre #a #pre1 #pre2 #post
-               (f : unit -> SteelT a pre1 post)
-               (_ : squash (pre1 == pre2)) :
-               (unit -> SteelT a pre2 post) = f
-
-val kfork : #p:hprop -> #q:hprop -> (unit -> steelK unit p (fun _ -> q)) -> steelK (thread q) p (fun _ -> emp)
-let kfork (#p:hprop) (#q:hprop) (f : unit -> steelK unit p (fun _ -> q))
-: steelK (thread q) p (fun _ -> emp)
+val kfork : #p:hprop -> #q:hprop -> (unit -> SteelK unit p (fun _ -> q)) -> SteelK (thread q) p (fun _ -> emp)
+let kfork (#p:hprop) (#q:hprop) (f : unit -> SteelK unit p (fun _ -> q))
+: SteelK (thread q) p (fun _ -> emp)
 =
-  assume (forall p. emp `star` p == p);
-  assume (forall p. p `star` emp == p);
+  SteelK?.reflect (
+  l_id ();
   fun (#frame:hprop) (#postf:hprop)
     (k : (x:(thread q) -> SteelT unit (frame `star` emp) (fun _ -> postf))) ->
     let t1 () : SteelT unit p (fun _ -> q) =
       let k : (unit -> SteelT unit q (fun _ -> q)) = fun () -> idk #q () in
-      f () #emp #q k
+      let r : steelK _ _ _ = reify (f ()) in 
+      reshuffle0 ();
+      r #emp #q (fun x -> reshuffle0 (); k x)
     in
-    let t2 (t:thread q) () : SteelT unit frame (fun _ -> postf) = k t in
+    let t2 (t:thread q) () : SteelT unit frame (fun _ -> postf) = reshuffle0 (); k t in
     let ff () : SteelT unit (p `star` frame) (fun _ -> postf)
               = fork #p #q #frame #postf t1 t2
     in
-    assume (star p frame == star frame p);
-    let ff2 : unit -> SteelT unit (star frame p) (fun _ -> postf) = change_pre ff () in
-    ff2 ()
+    l_comm ();
+    let ff2 : unit -> SteelT unit (star frame p) (fun _ -> postf) = change_pre ff in
+    ff2 ())
 
 (* just a flip of the usual frame *)
 assume val frame' : #a:_ -> #pre:_ -> #post:_ ->
@@ -73,55 +162,65 @@ assume val frame' : #a:_ -> #pre:_ -> #post:_ ->
                     (frame : hprop) ->
                     SteelT a (frame `star` pre) (fun x -> frame `star` (post x))
 
-let kjoin #p (t : thread p) : steelK unit emp (fun _ -> p) =
- fun #f k -> frame' (fun () -> join t) f; k ()
+let kjoin #p (t : thread p) : SteelK unit emp (fun _ -> p) =
+ SteelK?.reflect (fun #f k -> frame' (fun () -> join t) f; k ())
 
 val kframe : #a:Type -> #p:hprop -> #q:(post_t a) ->
              (f : hprop) ->
-             steelK a p q ->
-             steelK a (f `star` p) (fun x -> f `star` q x)
+             ($c : (unit -> SteelK a p q)) ->
+             SteelK a (f `star` p) (fun x -> f `star` q x)
 
-let kframe #a #p #q (f : hprop) (c : steelK a p q)
-  : steelK a (f `star` p) (fun x -> f `star` q x)
-  = fun #f0 #postf
+let kframe #a #p #q (f : hprop) ($c : (unit -> SteelK a p q))
+  : SteelK a (f `star` p) (fun x -> f `star` q x)
+  = SteelK?.reflect (fun #f0 #postf
       (k : (x:a -> SteelT unit (f0 `star` (f `star` q x)) (fun _ -> postf))) ->
-      assume (f0 `star` (f `star` p) == (f0 `star` f) `star` p);
-      assume (forall x. f0 `star` (f `star` q x) == (f0 `star` f) `star` q x);
+      l_assoc ();
+      l_comm (); (* blasting with AC.. seems to work fine *)
       let k' (x:a) : SteelT unit ((f0 `star` f) `star` q x) (fun _ -> postf) =
-          change_pre (fun () -> k x) () ()
+          change_pre (fun () -> k x) ()
       in
       let cc0 () : SteelT unit ((f0 `star` f) `star` p) (fun _ -> postf) =
-        c #(f0 `star` f) #postf k'
+        reify (c ()) #(f0 `star` f) #postf k'
       in
       let cc () : SteelT unit (f0 `star` (f `star` p)) (fun _ -> postf) =
-        change_pre cc0 () ()
+        change_pre cc0 ()
       in
-      cc ()
+      cc ())
 
 let cancel #p #q (c : steelK unit (p `star` emp) q) : steelK unit p q =
-  assume (p `star` emp == p);
-  c
+  l_id ();
+  subcomp _ _ _ _ _ c
 
 assume val q : int -> hprop
-assume val f : unit -> steelK unit emp (fun _ -> emp)
-assume val g : i:int -> steelK unit emp (fun _ -> q i)
-assume val h : unit -> steelK unit emp (fun _ -> emp)
+assume val f : unit -> SteelK unit emp (fun _ -> emp)
+assume val g : i:int -> SteelK unit emp (fun _ -> q i)
+assume val h : unit -> SteelK unit emp (fun _ -> emp)
 
-let example () : steelK unit emp (fun _ -> q 1 `star` q 2) =
-  assume (forall h. star h emp == h /\ star emp h == h);
-  let spawn2 (f : (x:int -> steelK unit emp (fun _ -> q x))) : steelK (thread (q 1) & thread (q 2)) emp (fun _ -> emp) =
-    pid1 <-- kfork (fun () -> f 1);
-    pid2 <-- kfork (fun () -> f 2);
-    return (pid1, pid2)
+private
+val reshufflek (#p #q : hprop)
+              (_ : squash (p `equiv` q))
+   : SteelK unit p (fun _ -> q)
+
+private
+let reshufflek #p #q peq =
+  ()
+  
+let example () : SteelK unit emp (fun _ -> q 1 `star` q 2) =
+  let spawn2 (f : (x:int -> SteelK unit emp (fun _ -> q x))) : SteelK (thread (q 1) & thread (q 2)) emp (fun _ -> emp) =
+    let pid1 = kfork (fun () -> f 1) in
+    let pid2 = kfork (fun () -> f 2) in
+    (pid1, pid2)
   in
-  f ();;
-  p1p2 <-- spawn2 g;
-  let (p1,p2) = p1p2 in
-  kjoin p1;;
-  kframe (q 1) begin
-    h ();;
-    kjoin p2;;
-    kframe (q 2) begin
-      return ()
-    end
-  end
+  f ();
+  let p1p2 = spawn2 g in
+  let p1 = fst p1p2 in
+  let p2 = snd p1p2 in
+  kjoin p1;
+  // GM: gah, I think I have to write it like this since SteelK doesn't really
+  // carry any logical payload, so lifts from pure things lose their spec.
+  let p : squash (equiv (q 1) (star (q 1) emp)) = forall_elim l_id (q 1) in
+  reshufflek ();
+  kframe (q 1) (fun () ->
+    h ();
+    kjoin p2
+  )
